finish st/left/union_insert.v, work on related case study

coq/st/left/union_insert.v
@@ -1,8 +1,11 @@
+Require Import Coq.Strings.String.
+Require Import CAS.coq.common.ast.
 Require Import CAS.coq.common.compute.
 Require Import CAS.coq.eqv.properties.
 Require Import CAS.coq.eqv.structures. 
 Require Import CAS.coq.eqv.set. 
-Require Import CAS.coq.sg.union. 
+Require Import CAS.coq.sg.union.
+Require Import CAS.coq.sg.cast_up. 
 Require Import CAS.coq.tr.left.insert.
 Require Import CAS.coq.bs.properties.
 Require Import CAS.coq.bs.union_union. 
@@ -49,7 +52,7 @@ Proof. destruct fin_d as [finP | nfinP].
          exact (@SLT_Id_Ann_Proof_Not_Equal _ _ _ _ _ A). 
        + exact (@SLT_Id_Ann_Proof_Id_None _ _ _ _ _ 
                    (bop_union_exists_id S eq ref sym trn,
-                    ltr_insert_not_exists_ann S eq wS f nt ref sym trn nfinP)).
+                    ltr_insert_not_exists_ann S eq ref sym trn nfinP)).
 Defined.          
 
 
@@ -66,5 +69,168 @@ let trn := A_eqv_transitive _ _ eqvP in
   A_left_semiring_distributive   := @slt_union_insert_distributive S eq ref sym trn 
 ; A_left_semiring_not_absorptive := @slt_union_insert_not_absorptive S wS eq 
 |}.
+
+Open Scope string_scope.
+
+
+Definition A_slt_union_insert (S :Type) (eqv : A_eqv S) :=
+let eq         := A_eqv_eq S eqv in
+let wS          := A_eqv_witness S eqv in
+let f          := A_eqv_new S eqv in
+let ntS        := A_eqv_not_trivial S eqv in
+let fin_d      := A_eqv_finite_d S eqv in
+let eqvP       := A_eqv_proofs S eqv in
+let refS       := A_eqv_reflexive _ _ eqvP in
+let symS       := A_eqv_symmetric _ _ eqvP in
+let trnS       := A_eqv_transitive _ _ eqvP in
+  {|
+    A_left_pre_semiring_carrier           := A_eqv_set S eqv 
+  ; A_left_pre_semiring_label             := eqv 
+  ; A_left_pre_semiring_plus              := bop_union eq 
+  ; A_left_pre_semiring_trans             := ltr_insert eq 
+  ; A_left_pre_semiring_plus_proofs       := (* ugh!  need some abstraction here....*)
+                                             A_sg_C_proofs_from_sg_CI_proofs
+                                               (finite_set S) 
+                                               (brel_set eq)
+                                               (bop_union eq) 
+                                               (wS :: nil)
+                                               (λ (l : finite_set S), if brel_set eq nil l then (wS :: nil) else nil)
+                                               (brel_set_not_trivial S eq wS)
+                                               (eqv_proofs_set S eq eqvP)
+                                               (sg_CI_proofs_union eqv)
+  ; A_left_pre_semiring_trans_proofs      := ltr_insert_proofs S eq wS f ntS eqvP 
+  ; A_left_pre_semiring_exists_plus_ann_d := bop_union_exists_ann_decide S eq refS symS trnS fin_d 
+  ; A_left_pre_semiring_id_ann_proofs_d   := slt_union_insert_exists_id_ann_decide S wS eq refS symS trnS fin_d 
+  ; A_left_pre_semiring_proofs            := union_insert_left_semiring_proofs S eq wS eqvP  
+  ; A_left_pre_semiring_ast               := Cas_ast ("slt_union_insert", (Cas_eqv_ast (A_eqv_ast _ eqv)) :: nil)
+|}.
+
  
 End ACAS.   
+
+Section AMCAS.
+
+
+Definition A_mcas_slt_union_insert (S : Type) (eqv : @A_mcas_eqv S) :=
+match eqv with
+| A_EQV_eqv A    => A_slt_classify (A_SLT_Left_Pre_Semiring (A_slt_union_insert _ A))
+| A_EQV_Error sl => A_SLT_Error sl     
+end.
+  
+End AMCAS.   
+
+Section CAS.
+
+Definition union_insert_left_semiring_certs {S : Type} (wS : S) :=
+{|
+  left_semiring_distributive   := Assert_Slt_Distributive 
+; left_semiring_not_absorptive := @Assert_Slt_Not_Absorptive S (finite_set S) (wS, nil) 
+|}.
+
+Open Scope string_scope.
+
+
+Definition slt_union_insert_exists_id_ann_certify {S : Type} (fin_d : @check_is_finite S) : @check_slt_exists_id_ann S (finite_set S) :=
+  match fin_d with
+  | Certify_Is_Finite enum => Certify_SLT_Id_Ann_Proof_Not_Equal (nil, enum tt)
+  | Certify_Is_Not_Finite  => Certify_SLT_Id_Ann_Proof_Id_None nil 
+  end. 
+  
+Definition slt_union_insert {S :Type} (eqv : @eqv S) :=
+let eq         := eqv_eq eqv in
+let wS         := eqv_witness eqv in
+let f          := eqv_new eqv in
+let fin_d      := eqv_finite_d eqv in
+  {|
+    left_pre_semiring_carrier           := eqv_set eqv 
+  ; left_pre_semiring_label             := eqv 
+  ; left_pre_semiring_plus              := bop_union eq 
+  ; left_pre_semiring_trans             := ltr_insert eq 
+  ; left_pre_semiring_plus_certs        := (* ugh!  need some abstraction here....*)
+                                             sg_C_certs_from_sg_CI_certs
+                                               (finite_set S) 
+                                               (brel_set eq)
+                                               (bop_union eq) 
+                                               (wS :: nil)
+                                               (λ (l : finite_set S), if brel_set eq nil l then (wS :: nil) else nil)
+                                               (sg_CI_certs_union eqv)
+  ; left_pre_semiring_trans_certs       := ltr_insert_certs wS f 
+  ; left_pre_semiring_exists_plus_ann_d := bop_union_exists_ann_certify fin_d 
+  ; left_pre_semiring_id_ann_certs_d    := slt_union_insert_exists_id_ann_certify fin_d 
+  ; left_pre_semiring_certs             := union_insert_left_semiring_certs wS
+  ; left_pre_semiring_ast               := Cas_ast ("slt_union_insert", (Cas_eqv_ast (eqv_ast eqv)) :: nil)
+|}.
+
+  
+  
+End CAS.
+
+Section MCAS.
+
+Definition mcas_slt_union_insert {S : Type} (eqv : @mcas_eqv S) :=
+match eqv with
+| EQV_eqv A    => slt_classify (SLT_Left_Pre_Semiring (slt_union_insert A))
+| EQV_Error sl => SLT_Error sl     
+end.
+  
+
+End MCAS.
+
+Section Verify.
+
+Lemma correct_id_ann_certs_union_insert
+      (S : Type)
+      (eq : brel S)
+      (wS : S)
+      (fin_d : carrier_is_finite_decidable S eq)
+      (ref : brel_reflexive S eq)
+      (sym : brel_symmetric S eq) 
+      (trn : brel_transitive S eq) : 
+     slt_union_insert_exists_id_ann_certify (p2c_is_finite_check S eq fin_d)
+     =
+     p2c_slt_exists_id_ann_check (brel_set eq) (bop_union eq) (ltr_insert eq)
+        (slt_union_insert_exists_id_ann_decide S wS eq ref sym trn fin_d). 
+Proof. unfold p2c_slt_exists_id_ann_check, slt_union_insert_exists_id_ann_decide,
+              slt_union_insert_exists_id_ann_certify, p2c_is_finite_check; 
+              destruct fin_d as [[enum A] | C]; simpl; reflexivity. 
+Qed.
+
+Lemma correct_certs_union_insert (S : Type) (eq : brel S) (wS : S) (eqvP : eqv_proofs S eq) :    
+      union_insert_left_semiring_certs wS 
+      = 
+      P2C_left_semiring (brel_set eq) (bop_union eq) (ltr_insert eq)
+        (union_insert_left_semiring_proofs S eq wS eqvP). 
+Proof. unfold union_insert_left_semiring_certs,
+       union_insert_left_semiring_proofs,
+       P2C_left_semiring; compute.
+       reflexivity. 
+Qed. 
+  
+Theorem correct_union_insert (S : Type) (eqv: A_eqv S) : 
+    slt_union_insert (A2C_eqv S eqv)
+    =
+    A2C_left_pre_semiring (A_slt_union_insert S eqv).
+Proof. unfold slt_union_insert, A_slt_union_insert, A2C_left_pre_semiring; simpl.
+       rewrite correct_eqv_set.
+       rewrite correct_bop_union_certs.
+       rewrite correct_ltr_certs_insert. 
+       rewrite <- correct_bop_union_exists_ann_certify.
+       rewrite <- correct_id_ann_certs_union_insert.       
+       rewrite <- correct_certs_union_insert.        
+       rewrite <- correct_sg_C_certs_from_sg_CI_certs.
+
+       reflexivity.
+Qed. 
+
+ 
+Theorem correct_bop_mcas_union_insert (S : Type) (eqvS : @A_mcas_eqv S): 
+         mcas_slt_union_insert (A2C_mcas_eqv S eqvS)  
+         = 
+         A2C_mcas_slt (A_mcas_slt_union_insert S eqvS). 
+Proof. destruct eqvS; simpl.
+       + reflexivity. 
+       + rewrite correct_union_insert.
+         apply correctness_slt_classify_left_pre_semiring_slt. 
+Qed.  
+
+End Verify.   
